Rake: introduce HasNonMultiple

Rake.lean
@@ -253,7 +253,7 @@ end « partition »
 
 section « rem (remove multiples) »
 
-variable (r: Rake) (j: Nat) (hj: 0<j)
+variable (r: Rake) {j: Nat} (hj: 0<j)
 
 /-- remove all multiples of `j`. -/
 def rem : Rake :=
@@ -267,21 +267,22 @@ def rem : Rake :=
   if hlen: ks.length = 0 then zer
   else { d := r'.d, ks:=ks, sorted := false, hsize := Nat.zero_lt_of_ne_zero hlen }
 
-variable (r':Rake) (hr': r' = r.rem j hj)
+abbrev HasNonMultiple (j:Nat): Prop := ∃n, ¬j∣n ∧ ∃m, r.term m=n
+variable {r': Rake} (hr': r' = r.rem hj)
 
 lemma rem_def'
   : r'=zer
   ∨ (r'.d=r.d*j ∧ r'.ks=(r.partition j hj).ks.filter (λk => ¬j∣k) ∧ 0<r'.ks.length) := by
     simp[hr',rem,partition]; split <;> simp_all[Nat.zero_lt_of_ne_zero]
 
-theorem rem_def  (h₁: ∃n, ¬j∣n ∧ ∃m, r.term m=n)
+theorem rem_def (hnm: HasNonMultiple r j)
   : r'.d=r.d*j ∧ r'.ks=(r.partition j hj).ks.filter (λk => ¬j∣k) ∧ 0<r'.ks.length := by
-  obtain hzer | ⟨hd', hks', hlen'⟩ := rem_def' r j hj r' hr'
+  obtain hzer | ⟨hd', hks', hlen'⟩ := rem_def' r hj hr'
   · -- show hzer case cannot happen thanks to h₁
     -- r produces terms that don't divide k, and r.partition produces the same terms.
 
     -- from h1 we can obtain a k∈r.k coprime to p
-    obtain ⟨n, hn, hex⟩ := h₁
+    obtain ⟨n, hn, hex⟩ := hnm
     obtain ⟨k, hk, x, hx⟩ := by rwa[←r.partition_term_iff j hj n, term_iff] at hex
     have hjk : ¬j ∣ k := by
       by_contra h
@@ -312,32 +313,27 @@ theorem rem_def  (h₁: ∃n, ¬j∣n ∧ ∃m, r.term m=n)
   · -- the other case (non hzer) just passes right through
     exact ⟨hd', hks', hlen'⟩
 
-theorem rem_drop  -- rem drops multiples of p
-  : 0<n → j∣n → ¬(∃m, r'.term m = n) := by
+theorem rem_drop (hnm: HasNonMultiple r j) -- rem drops multiples of p
+  : j∣n → ¬(∃m, r'.term m = n) := by
   -- general idea:
   --   the only way term m = n is if ∃x, ∃k∈r.ks, k + x*d = n
   --   x would have to be be n/ks.length, but i'm not sure we need that fact
   --   term_iff supplies this fact.
-  intro hnpos hpn; rw[term_iff]
+  intro hpn; rw[term_iff]
   -- we will show no such k exists
   push_neg; intro k hk x
   set d' := r'.d
   -- either rem returns zer, or we can extract the formulas for d and ks
-  obtain hzer | ⟨hd', hks', hlen'⟩ := rem_def' r j hj r' hr'
-  · -- the r=zer case solves the whole issue because zer only ever returns zero
-    subst hzer
-    have : k = 0 := by simp[zer] at hk; exact hk
-    have : d' = 0 := by simp[d',zer]
-    simp_all; exact Nat.ne_of_lt hnpos
-  · -- we only have to show ¬p∣k, because `p∣d` so `x*d` cancels out mod p
-    suffices ¬j∣k from by
-      by_contra h
-      have h₀: j ∣ k + x * d' := by rwa[h.symm] at hpn
-      have h₁: j ∣ x * d' := Dvd.dvd.mul_left (Dvd.intro_left r.d hd'.symm) x
-      have : j ∣ k := (Nat.dvd_add_iff_left h₁).mpr h₀
-      contradiction
-    show ¬j∣k
-    simp_all[List.mem_filter]
+  obtain ⟨hd', hks', hlen'⟩ := rem_def r hj hr' hnm
+  -- we only have to show ¬j∣k, because `j∣d` so `x*d` cancels out mod j
+  suffices ¬j∣k from by
+    by_contra h
+    have h₀: j ∣ k + x * d' := by rwa[h.symm] at hpn
+    have h₁: j ∣ x * d' := Dvd.dvd.mul_left (Dvd.intro_left r.d hd'.symm) x
+    have : j ∣ k := (Nat.dvd_add_iff_left h₁).mpr h₀
+    contradiction
+  show ¬j∣k
+  simp_all[List.mem_filter]
 
 theorem rem_keep  -- rem keeps non-multiples of p
   : ¬j∣n → (∃m, r.term m = n) → (∃m', r'.term m' = n) := by
@@ -348,8 +344,8 @@ theorem rem_keep  -- rem keeps non-multiples of p
   rw[←r.partition_term_iff j hj n, term_iff] at ht'
   -- since r.partition produces n, we can show ¬p∣k for the corresponding k
   obtain ⟨k, hk, x, hx⟩ := ht'
-  have hex : (∃n, ¬j∣n ∧ ∃m, r.term m = n) := by use n
-  obtain ⟨hd', hks'⟩ := rem_def r j hj r' hr' hex
+  have hnm: HasNonMultiple r j := by use n
+  obtain ⟨hd', hks'⟩ := rem_def r hj hr' hnm
   -- !! this duplicates some work from rem_def' ... consolidate?
   have hpk : ¬ j ∣ k := by
     by_contra h
@@ -365,11 +361,11 @@ theorem rem_keep  -- rem keeps non-multiples of p
   rw[term_iff]
   use k; aesop
 
-theorem rem_same  -- rem introduces no new terms
-  : (∃n, ¬j∣n ∧ ∃m, r.term m = n) → (∃m', r'.term m' = n) → (∃m, r.term m = n) := by
+theorem rem_same (hnm: HasNonMultiple r j) -- rem introduces no new terms
+  : (∃m', r'.term m' = n) → (∃m, r.term m = n) := by
   -- this follows from partition_term_iff and the nature of filter.
-  intro hex h; rw[term_iff] at h; obtain ⟨k, hk, x, hx⟩ := h
-  obtain ⟨hd', hks'⟩ := rem_def r j hj r' hr' hex
+  intro h; rw[term_iff] at h; obtain ⟨k, hk, x, hx⟩ := h
+  obtain ⟨hd', hks'⟩ := rem_def r hj hr' hnm
   have := r.partition_term_iff j hj n
   rw[term_iff] at this; rw[←this]
   have : k ∈ (r.partition j hj).ks := by simp_all; exact List.mem_of_mem_filter hk
